Commit of the Week

theories/Commons/Language.v
@@ -1,17 +1,18 @@
 From RSL Require Import Prelude.
-From RSL Require Export Commons.Memory.
+
+From RSL.Commons Require Export Memory Values.
 
 Section lang_mixin.
   Context {prog pstate value : Type}.
 
   Context (step_rel : prog -> (pstate * memory) -> (pstate * memory) -> Prop).
-  Context (is_final : (pstate * memory) -> option (value * memory)).
+  Context (is_value : pstate -> option value).
 
   Record LangMixin := {
       mixin_final_no_step:
-      ∀ s v m,
-        is_final s = Some (v, m) ->
-        ∀ p s', ~step_rel p s s';
+      ∀ s v,
+        is_value s = Some v ->
+        ∀ m p s', ~step_rel p (s, m) s';
     }.
 End lang_mixin.
 
@@ -23,13 +24,13 @@ Structure lang :=
       value : Type;
 
       step_rel : prog -> (pstate * memory) -> (pstate * memory) -> Prop;
-      is_final : (pstate * memory) -> option (value * memory);
+      is_value : pstate -> option value;
 
-      lang_mixin : LangMixin step_rel is_final;
+      lang_mixin : LangMixin step_rel is_value;
     }.
 
 Arguments step_rel {_} _ _ _.
-Arguments is_final {_} _.
+Arguments is_value {_} _.
 
 Notation "P ⊨ s '->>' t" := (step_rel P s t) (at level 60, right associativity).
 Notation "P ⊨ s '-{' n '}>' t" := (nsteps (step_rel P) n s t) (at level 60, right associativity).
@@ -41,22 +42,54 @@ Definition state (Λ: lang) : Type := pstate Λ * memory.
 Definition pstate_of_state {Λ : lang} : state Λ -> pstate Λ := fst.
 Definition memory_of_state {Λ : lang} : state Λ -> memory := snd.
 
+Definition is_final {Λ : lang} (s: state Λ) :=
+  let '(ps, m) := s in
+  match is_value ps with
+  | Some v => Some (v, m)
+  | None => None
+  end.
+
 Section LangProp.
   Context {Λ: lang} (P: prog Λ).
+  Implicit Type s : state Λ.
+  Implicit Type v : value Λ.
+
+  Lemma is_final_Some s v m:
+    is_final s = Some (v, m)
+    <->
+      ∃ ps, s = (ps, m) ∧ is_value ps = Some v.
+  Proof using Type.
+    split.
+    - destruct s as [ps ?]. simpl.
+      destruct (is_value ps) eqn:Hp; intros H; inv H.
+      eexists. by split.
+    - intros (ps & -> & Hfin). simpl. by rewrite Hfin.
+  Qed.
+
+  Local Lemma is_final_None s:
+    is_final s = None
+    <->
+      ∃ ps m, s = (ps, m) ∧ is_value ps = None.
+  Proof using Type.
+    split.
+    - destruct s as [ps m]. simpl.
+      destruct (is_value ps) eqn:Hp; intros H; inv H.
+      eexists ps, m. by split.
+    - intros (ps & m & -> & Hfin). simpl. by rewrite Hfin.
+  Qed.
 
   Lemma final_no_step s:
     is_Some (is_final s) -> ∀ t, ~(P ⊨ s ->> t).
   Proof using Type.
-    intros [[] Hf] t. eapply mixin_final_no_step.
+    intros [[] (ps & -> & Hfin)%is_final_Some] t.
+    eapply mixin_final_no_step.
     - apply lang_mixin.
-    - exact Hf.
+    - exact Hfin.
   Qed.
 
-  Definition can_progress (s: state Λ): Prop :=
-    ∃ t, P ⊨ s ->> t.
+  Definition can_progress s: Prop := ∃ t, P ⊨ s ->> t.
 
-  Definition stuck (s: state Λ) : Prop :=
-    is_final s = None ∧ ~ can_progress s.
+  Definition stuck s : Prop := is_final s = None ∧ ~ can_progress s.
 
   Lemma can_progress_must_step s:
     can_progress s -> ∃ t, P ⊨ s ->> t.
@@ -65,10 +98,11 @@ Section LangProp.
   Lemma final_no_progress s:
     is_Some (is_final s) -> ~can_progress s.
   Proof using Type.
-    intros [[] Hfin] Hp. destruct (can_progress_must_step _ Hp) as (? & H).
+    intros [[] (ps & -> & Hfin)%is_final_Some] Hp.
+    destruct (can_progress_must_step _ Hp) as (? & H).
     eapply mixin_final_no_step.
     - apply lang_mixin.
-    - eassumption.
+    - exact Hfin.
     - exact H.
   Qed.
 
@@ -81,6 +115,21 @@ Section LangProp.
   Lemma progress_not_stuck s:
     can_progress s -> ~ stuck s.
   Proof using Type. intros H [_ Hnprog]. by eapply Hnprog. Qed.
+
+  Lemma is_final_mem_ignore ps m m1 m2 v :
+    is_final (ps, m1) = Some (v, m) ->
+    is_final (ps, m2) = Some (v, m2).
+  Proof using Type.
+    intros (? & He & Hfin)%is_final_Some.
+    inv He. simpl. by rewrite Hfin.
+  Qed.
+
+  Lemma is_final_mem_same ps m m' v :
+    is_final (ps, m) = Some (v, m') ->
+    m = m'.
+  Proof using Type.
+    intros (? & He & Hfin)%is_final_Some. by inv He.
+  Qed.
 End LangProp.
 
 Section TwoProg.
