theories/Commons/Memory.v
@@ -1,34 +1,66 @@
-From Stdlib Require Import ZArith.
+From RSL Require Import Prelude.
+
+From RSL.Commons Require Export Values.
 
 From stdpp Require Import gmap.
-
-Definition val : Type := Z.
-Definition loc : Type := positive.
+From stdpp Require Export fin_maps.
 
 (* [memory] is a mapping from location to a value *)
 Definition memory := (gmap loc val).
 
 Instance memory_inhabited : Inhabited memory := populate ∅.
 
-Definition loc_to_val (l: loc) : val := Zpos l.
-
-Definition val_to_loc (v: val) : option loc :=
-  if (v >=? 1)%Z
-  then Some (Z.to_pos v)
-  else None.
-
 Definition get_at (addr: val) (m: memory) : option val :=
-  match val_to_loc addr with
-  | Some l => m !! l
-  | None => None
+  match addr with
+  | VPtr l => m !! l
+  | _ => None
   end.
 
 Definition set_at (addr: val) (v: val) (m: memory) : option memory :=
-  match val_to_loc addr with
-  | Some l =>
+  match addr with
+  | VPtr l =>
       match m !! l with
       | None => None
-      | Some _ => Some (alter (fun _ => v) l m)
+      | Some _ => Some (<[l := v]> m)
       end
-  | None => None
+  | _ => None
   end.
+
+Lemma get_at_union_left l (m1 m2: memory) :
+  m2 !! l = None ->
+  get_at (VPtr l) (m1 ∪ m2) = get_at (VPtr l) m1.
+Proof.
+  intros Hmem; simpl. by apply lookup_union_l.
+Qed.
+
+Lemma get_at_union_right l (m1 m2: memory) :
+  m1 !! l = None ->
+  get_at (VPtr l) (m1 ∪ m2) = get_at (VPtr l) m2.
+Proof.
+  intros Hmem; simpl. by apply lookup_union_r.
+Qed.
+
+Lemma get_at_singl l v :
+  get_at (VPtr l) {[ l := v ]} = Some v.
+Proof.
+  now apply lookup_singleton_eq.
+Qed.
+
+Lemma set_at_some l v old m:
+  get_at (VPtr l) m = Some old ->
+  set_at (VPtr l) v m = Some (<[l := v]> m).
+Proof.
+  unfold set_at, get_at.
+  intros Hget.
+  destruct (m !! l) as [[]|]; congruence.
+Qed.
+
+Lemma set_at_none addr v m:
+  get_at addr m = None ->
+  set_at addr v m = None.
+Proof.
+  unfold set_at, get_at.
+  intros Hget.
+  destruct addr; auto.
+  by rewrite Hget.
+Qed.
