theories/Simulations/FreeSimRules.v
@@ -2,167 +2,209 @@ From RSL Require Import Prelude.
 
 From Coinduction Require Import all.
 
-From RSL Require Import Simulations.FreeSim.
-From RSL Require Import Simulations.Equiv.
+From RSL.Simulations Require Export FreeSim.
+
+From RSL.Logic Require Export BI.
+From RSL.Logic Require Import rPropDef.
 
 Section FSimRules.
   Context {Λₜ Λₛ: lang}.
-  Context (J I: WfRel).
   Context (Pₜ: prog Λₜ) (Pₛ: prog Λₛ).
 
-  Abbreviation fsim := (fsim J I Pₜ Pₛ).
-  Abbreviation fsim_lfp := (fsim_lfp J I Pₜ Pₛ).
+  Abbreviation fsim := (fsim WfNat WfNat Pₜ Pₛ).
+  Abbreviation fsim_lfp := (fsim_lfp WfNat WfNat Pₜ Pₛ).
+  Abbreviation post := (value Λₜ -> value Λₛ -> rProp).
 
-  Implicit Types (C: Chain fsim_lfp).
+  Implicit Types (C: Chain fsim_lfp) (ϕ: post).
 
-  Lemma fsim_in_chain Post:
-    ∀ t j i s,
-    (∀ C, fsim_lfp (elem C) Post t j i s) ->
-    fsim Post t j i s.
+  Definition sim_lfp C st j i ss ϕ : rProp :=
+    {|
+      rProp_holds mt ms :=
+        let Ψ '(vt, mt) '(vs, ms) := rProp_holds (ϕ vt vs) mt ms in
+        fsim_lfp (elem C) Ψ (st, mt) j i (ss, ms)
+    |}.
+
+  Definition sim st j i ss ϕ : rProp :=
+    {|
+      rProp_holds mt ms :=
+        let Ψ '(vt, mt) '(vs, ms) := rProp_holds (ϕ vt vs) mt ms in
+        fsim Ψ (st, mt) j i (ss, ms)
+    |}.
+
+  Notation
+    "'[' C ']' st '<{' j ',' i '}=' ss '{{' Q '}}'" :=
+    (sim_lfp C st j i ss Q%I)
+      (at level 0, st at level 0, ss at level 0, no associativity).
+
+  Notation
+    "st '<{' j ',' i '}=' ss '{{' Q '}}'" :=
+    (sim st j i ss Q%I)
+      (at level 1, ss at level 1, no associativity).
+
+  Lemma fsim_in_chain st j i ss ϕ:
+    (∀ C, [C] st <{j, i}= ss {{ ϕ }}) -∗
+    st <{j, i}= ss {{ ϕ }}.
   Proof using Type.
-    intros t j i s Hr.
-    unfold fsim.
+    unseal.
+    intros ? ? [-> ->] mt ms _ _ H.
+    rewrite !map_empty_union.
+    unfold sim, sim_lfp, fsim.
     apply (gfp_prop).
-    intros C.
-    apply (b_chain C), Hr.
+    intros C. simpl.
+    apply (b_chain C), H.
   Qed.
 
-  Lemma final C Post:
-    ∀ t j i s,
-    both_final Post t s ->
-    elem C Post t j i s.
+  Lemma final C st j i ss ϕ:
+    ∀ vt vs,
+    ⌜is_value st = Some vt⌟ -∗
+    ⌜is_value ss = Some vs⌟ -∗
+    ϕ vt vs -∗
+    [C] st <{j, i}= ss {{ ϕ }}.
   Proof using Type.
-    apply tower.
-    { intros P Hp t j i s H Q Hq. eapply Hp; now eauto. }
-    intros C' CIH t j i s H. econstructor; now eauto.
-  Qed.
-
-  Lemma stuck C Post:
-    ∀ t j i s,
-    stuck Pₛ s ->
-    elem C Post t j i s.
-  Proof using Type.
-    apply tower.
-    { intros P Hp t j i s H Q Hq. eapply Hp; now eauto. }
-    intros C' CIH t j i s H. econstructor; now eauto.
-  Qed.
-
-  Lemma source_step C Post:
-    ∀ j t i i' s s',
-    Pₛ ⊨ s ->> s' ->
-    elem C Post t j i' s' ->
-    elem C Post t j i s.
-  Proof using Type.
-    apply tower.
-    { intros P Hp t j i i' s s' Hstep H Q Hq. eapply Hp; now eauto. }
-    intros C' CIH t j i i' s s' Hstep H. econstructor; now eauto.
-  Qed.
-
-  Lemma target_step C Post:
-    ∀ t j i s,
-    can_progress Pₜ t ->
-    (∀ t', Pₜ ⊨ t ->> t' -> ∃ j', elem C Post t' j' i s) ->
-    elem C Post t j i s.
-  Proof using Type.
-    apply tower.
-    { intros P Hp t j i s Hprogesss H Q Hq.
-      eapply Hp; eauto.
-      intros t' Hstep. destruct (H _ Hstep) as [j' Hinf].
-      exists j'. now auto. }
-    intros C' CIH t j i s Hprogress Ht. econstructor; now eauto.
-  Qed.
-
-  Lemma progress_step C Post:
-    ∀ t j j' i i' s,
-    j' ⊏ j ->
-    i' ⊏ i ->
-    elem C Post t j' i' s ->
-    elem C Post t j i s.
-  Proof using Type.
-    apply tower.
-    { intros P Hp t j j' i i' s Ht Hs H Q Hq.
-      eapply Hp; now eauto. }
-    intros C' CIH t j j' i i' s Ht Hs H.
-    eapply FProgress; try eassumption.
-    now apply (b_chain C').
-  Qed.
-
-  Lemma coind_weak C Post:
-    ∀ t j i s,
-    (∀ C,
-       (∀ j' i', j ⊏ j' -> i ⊏ i' -> fsim_lfp (elem C) Post t j' i' s) ->
-       fsim_lfp (elem C) Post t j i s) ->
-    elem C Post t j i s.
-  Proof using Type.
-    intros t j i s RIH.
-    apply tower.
-    { intros P Hp Q Hq. eapply Hp; now eauto. }
-    intros C' CIH.
-    apply RIH. intros j' i' Hj Hi.
-    eapply FProgress; now eauto.
-  Qed.
-
-  Lemma coind_strong C Post (Inv: _ -> state Λₜ -> J -> I -> state Λₛ -> Prop) :
-    (∀ C t j i s,
-       (∀ j' t i' s,
-          Inv Post t j i s ->
-          j ⊏ j' ->
-          i ⊏ i' ->
-          fsim_lfp (elem C) Post t j' i' s) ->
-       Inv Post t j i s ->
-       fsim_lfp (elem C) Post t j i s) ->
-    ∀ t j i s,
-    Inv Post t j i s ->
-    elem C Post t j i s.
-  Proof using Type.
-    intros RIH.
-    apply tower.
-    { intros Z Hz t j i s HP Q Hq. eapply Hz; now eauto. }
-    intros C' CIH t j i s HP.
-    apply RIH.
-    - intros t' j' i' s' HP' Hj Hi.
-      eapply FProgress; now eauto.
+    unseal.
+    intros vt vs ? ? [-> ->].
+    intros ? ? _ _ [[-> ->] Ht].
+    intros ? ? _ _ [[-> ->] Hs].
+    intros mt ms _ _ Hp. rewrite !map_empty_union.
+    apply FRelated.
+    eexists _, _. split_and!.
+    - simpl. by rewrite Ht.
+    - simpl. by rewrite Hs.
     - assumption.
   Qed.
 
-  Lemma coind_weak_open Post:
-    ∀ t j i s,
-    (∀ R,
-       (∀ j' i',
-          j ⊏ j' ->
-          i ⊏ i' ->
-          fsim_lfp R Post t j' i' s) ->
-       fsim_lfp R Post t j i s) ->
-    fsim_lfp fsim Post t j i s.
+  Lemma sim_mono C st j i ss ϕ:
+    ∀ j' i' ϕ',
+    □ (∀ vt vs, ϕ' vt vs -∗ ϕ vt vs) -∗
+    ⌜j' ⊑ j⌟ -∗
+    ⌜i' ⊑ i⌟ -∗
+    [C] st <{j', i'}= ss {{ ϕ' }} -∗
+    [C] st <{j, i}= ss {{ ϕ }}.
   Proof using Type.
-    intros t j i s RIH.
-    apply fsim_unroll.
-    coinduction C CIH.
-    apply RIH. intros j' i' Hj Hi.
-    eapply FProgress; now eauto.
+    revert st j i ss ϕ.
+    unseal. unfold sim_lfp.
+    apply tower.
+    { intros P Hp. do 30 intro. intros Hinf Q Hq.
+      eapply (Hp _ Hq); eauto. by apply Hinf. }
+    clear C. intros C CIH.
+    intros st j i ss ϕ j' i' ϕ' ? ? [-> ->] mtP msP _ _ [[-> ->] Hϕ].
+    intros ? ? _ _ [[-> ->] Hj] ? ? _ _ [[-> ->] Hi].
+    intros mt ms _ _ H.
+    simpl in H, Hj, Hi, Hϕ.
+    remember (st, mt : memory) as t eqn:Ht.
+    remember (ss, ms : memory) as s eqn:Hs.
+    revert i j st mt ss ms Hj Hi Hϕ CIH Ht Hs.
+    induction H as
+      [ t j' i' s Hfin
+      | t j' i' s Hstuck
+      | t j' i'' i' s s' Hstep Hsim IHs
+      | t j' i' s Hprogress IHt
+      | t j' j'' i' i'' s Ht Hs Hgfp ].
+    - intros i j st mt ss ms Hj Hi Hϕ _ -> ->.
+      apply FRelated.
+      destruct Hfin as ([] & [] &
+                          (vt & Het & Hft)%is_final_Some &
+                          (vs & Hes & Hfs)%is_final_Some & Hfin). subst.
+      inv Het.
+      eexists _, _. split_and!.
+      + unfold is_final. by rewrite Hft.
+      + unfold is_final. by rewrite Hfs.
+      + apply Hϕ.
+        * by rewrite !map_empty_union.
+        * by rewrite !map_empty_union; apply map_disjoint_empty_r.
+        * by rewrite !map_empty_union; apply map_disjoint_empty_r.
+        * assumption.
+    - intros i j st mt ss ms Hj Hi Hϕ _ -> ->.
+      apply FSourceStuck. by rewrite !map_empty_union.
+    - intros i j st mt ss ms Hj Hi Hϕ CIH -> ->.
+      destruct s' as [ss' ms'].
+      eapply FSourceSteps with (s' := (ss', ∅ ∪ ∅ ∪ ∅ ∪ ∅ ∪ ms')) (i' := i').
+      { by rewrite !map_empty_union. }
+      by apply IHs.
+    - intros i j st mt ss ms Hj Hi Hϕ CIH -> ->.
+      apply FTargetSteps. { by rewrite !map_empty_union. }
+      intros [st' mt'] Ht'.
+      rewrite !map_empty_union in Ht'.
+      apply IHt in Ht' as (j'' & Hsim & IH).
+      exists j''.
+      replace mt' with (∅ ∪ ∅ ∪ ∅ ∪ ∅ ∪ mt') by now rewrite !map_empty_union.
+      by apply IH.
+    - intros i j st mt ss ms Hj Hi Hϕ CIH -> ->.
+      destruct Hj as [Hj | ->], Hi as [Hi | ->];
+      (eapply FProgress; try done; eapply CIH; clear CIH; try done);
+      try (rewrite !map_empty_union; apply map_disjoint_empty_r);
+      (split; [done | simpl]); auto; now left.
   Qed.
 
-  Lemma coind_strong_open Post (Inv: _ -> state Λₜ -> J -> I -> state Λₛ -> Prop) :
-    (∀ R t j i s,
-       (∀ j' t i' s,
-          Inv Post t j i s ->
-          j ⊏ j' ->
-          i ⊏ i' ->
-          fsim_lfp R Post t j' i' s) ->
-       Inv Post t j i s ->
-       fsim_lfp R Post t j i s) ->
-    ∀ t j i s,
-    Inv Post t j i s ->
-    fsim_lfp fsim Post t j i s.
+  Lemma coind C Inv:
+    □ (∀ C st j i ss ϕ,
+       □ (∀ st' j' i' ss' ϕ',
+            ⌜j ⊏ j'⌟ -∗
+            ⌜i ⊏ i'⌟ -∗
+            Inv st' j i ss' ϕ' -∗
+            [C] st' <{j', i'}= ss' {{ ϕ' }}) -∗
+       Inv st j i ss ϕ -∗
+       [C] st <{j, i}= ss {{ ϕ }}) -∗
+    ∀ st j i ss ϕ,
+    Inv st j i ss ϕ -∗
+    [C] st <{j, i}= ss {{ ϕ }}.
   Proof using Type.
-    intros RIH t j i s HP.
-    apply fsim_unroll.
-    revert t j i s HP.
-    coinduction C CIH.
-    intros t j i s HP.
-    apply RIH.
-    - intros j' t' i' s' Hj Hi HP'.
-      eapply FProgress; now eauto.
-    - assumption.
+    unseal. unfold sim_lfp.
+    intros ? ? [-> ->] ? ? _ _ [[-> ->] RIH].
+    apply tower.
+    { intros P Hp. do 9 intro. intros Hinf Q Hq. by apply (Hp _ Hq). }
+    clear C. intros C CIH.
+    intros st j i ss ϕ mtI msI _ _ HI. simpl.
+    apply RIH; clear RIH.
+    - by split.
+    - easy.
+    - easy.
+    - split; [done |]. simpl.
+      intros ? ? [-> ->] st' i' j' ss' ϕ'.
+      intros ? ? _ _ [[-> ->] Hj].
+      intros ? ? _ _ [[-> ->] Hi].
+      intros mt ms _ _ HInv.
+      eapply FProgress; [done | done |].
+      apply CIH; auto; by rewrite !map_empty_union; apply map_disjoint_empty_r.
+    - by rewrite !map_empty_union; apply map_disjoint_empty_r.
+    - by rewrite !map_empty_union; apply map_disjoint_empty_r.
+    - easy.
+  Qed.
+
+  Definition hoare P st ss Q : rProp :=
+    □ (∀ ϕ,
+         P -∗
+         (∀ vt vs, Q vt vs -∗ ϕ vt vs) -∗
+         st <{0, 0}= ss {{ϕ}})%I.
+
+  Notation
+    "'{{' P '}}' st '≲' ss '{{' Q '}}'" :=
+    (hoare P%I st ss Q%I)
+      (at level 0, st at level 0, ss at level 0, no associativity).
+
+  Lemma frame P1 P2 st ss Q :
+    {{ P1 }} st ≲ ss {{ Q }} -∗
+    {{ P1 ∗ P2 }} st ≲ ss {{ fun vt vs => Q vt vs ∗ P2 }}.
+  Proof using Type.
+    iIntros "#H !>" (ϕ) "[H1 H2] Hp".
+    iApply ("H" with "H1").
+    iIntros (vt vs) "Hq".
+    iApply "Hp". iFrame.
+  Qed.
+
+  Lemma consequence C P st ss Q :
+    ∀ P' Q',
+    □ (P -∗ P') -∗
+    □ (∀ vt vs, Q' vt vs -∗ Q vt vs) -∗
+    {{ P' }} st ≲ ss {{ Q' }} -∗
+    {{ P }} st ≲ ss {{ Q }}.
+  Proof using Type.
+    iIntros (P' Q') "#HP #HQ #H !>".
+    iIntros (ϕ) "Hpre Hpost".
+    iApply ("H" with "[Hpre] [Hpost]").
+    - by iApply "HP".
+    - iIntros (vt vs) "HQ'".
+      iApply "Hpost".
+      by iApply "HQ".
   Qed.
 End FSimRules.
