theories/Commons/BijSet.v
@@ -1,0 +1,123 @@
+From RSL Require Import Prelude.
+
+From stdpp Require Import gmap.
+
+Section bij_set.
+  Context `{Countable A, Countable B}.
+  Implicit Types (a : A) (b : B).
+
+  Definition bij_set (L : gset (A * B)) :=
+    ∀ a b,
+    (a, b) ∈ L ->
+    (∀ b', (a, b') ∈ L -> b' = b) ∧
+    (∀ a', (a', b) ∈ L -> a' = a).
+
+  Lemma bij_set_empty : bij_set ∅.
+  Proof using Type. by intros ?? []%not_elem_of_empty. Qed.
+
+  Lemma bij_set_extend L a b :
+    bij_set L ->
+    (∀ b', (a, b') ∉ L) ->
+    (∀ a', (a', b) ∉ L) ->
+    bij_set ({[(a, b)]} ∪ L).
+  Proof using Type.
+    intros Hbij Ha Hb a' b' [He%elem_of_singleton|Hin]%elem_of_union.
+    - inv He. split.
+      + intros ? [He%elem_of_singleton|Hin]%elem_of_union.
+        * by inv He.
+        * exfalso. by eapply Ha.
+      + intros ? [He%elem_of_singleton|Hin]%elem_of_union.
+        * by inv He.
+        * exfalso. by eapply Hb.
+    - split.
+      + intros ? [He%elem_of_singleton|Hin']%elem_of_union.
+        * exfalso. by inv He; eapply Ha.
+        * by eapply Hbij.
+      + intros ? [He%elem_of_singleton|Hin']%elem_of_union.
+        * exfalso. by inv He; eapply Hb.
+        * by eapply Hbij.
+  Qed.
+
+  Lemma bij_set_eq_iff L a1 a2 b1 b2 :
+    bij_set L ->
+    (a1, b1) ∈ L ->
+    (a2, b2) ∈ L ->
+    a1 = a2 <-> b1 = b2.
+  Proof using Type.
+    intros HL H1 H2.
+    destruct (HL _ _ H1) as [Hb1 Ha1].
+    split; intros ->.
+    - by rewrite (Hb1 _ H2).
+    - by rewrite (Ha1 _ H2).
+  Qed.
+
+  Lemma bij_set_subseteq L L' :
+    bij_set L -> L' ⊆ L -> bij_set L'.
+  Proof using Type.
+    intros Hbij Hle a b Hin.
+    split.
+    - intros ? Hin'. eapply Hbij; eapply elem_of_subseteq; eassumption.
+    - intros ? Hin'. eapply Hbij; eapply elem_of_subseteq; eassumption.
+  Qed.
+
+  Lemma bij_set_functional L a b1 b2 :
+    bij_set L ->
+    (a, b1) ∈ L ->
+    (a, b2) ∈ L ->
+    b1 = b2.
+  Proof using Type.
+    intros Hbij H1 H2. by erewrite <-bij_set_eq_iff.
+  Qed.
+
+  Lemma bij_set_injective L a1 a2 b :
+    bij_set L ->
+    (a1, b) ∈ L ->
+    (a2, b) ∈ L ->
+    a1 = a2.
+  Proof using Type.
+    intros Hbij H1 H2. by erewrite ->bij_set_eq_iff.
+  Qed.
+
+  Lemma bij_set_intersection  L1 L2 :
+    bij_set L1 -> bij_set (L1 ∩ L2).
+  Proof using Type.
+    intros Hbij1 a b [H1 _]%elem_of_intersection. split.
+    - intros b' [H2 _]%elem_of_intersection.
+      by eapply bij_set_functional.
+    - intros a' [H2 _]%elem_of_intersection.
+      by eapply bij_set_injective.
+  Qed.
+
+  Lemma bij_set_diff L1 L2 :
+    bij_set L1 -> bij_set (L1 ∖ L2).
+  Proof using Type.
+    intros Hbij a b [H1 _]%elem_of_difference. split.
+    - intros b' [H2 _]%elem_of_difference.
+      by eapply bij_set_functional.
+    - intros a' [H2 _]%elem_of_difference.
+      by eapply bij_set_injective.
+  Qed.
+
+  Lemma bij_set_diff_fst_neq L a1 a2 b1 b2 :
+    bij_set L ->
+    (a1, b1) ∈ L ->
+    (a2, b2) ∈ L ∖ {[ (a1, b1) ]} ->
+    a1 ≠ a2.
+  Proof using Type.
+    intros Hbij H1 [H2 Hneq%not_elem_of_singleton]%elem_of_difference.
+    intros ->. apply Hneq.
+    f_equal. by eapply bij_set_functional.
+  Qed.
+
+  Lemma bij_set_diff_snd_neq L a1 a2 b1 b2 :
+    bij_set L ->
+    (a1, b1) ∈ L ->
+    (a2, b2) ∈ L ∖ {[ (a1, b1) ]} ->
+    b1 ≠ b2.
+  Proof using Type.
+    intros Hbij H1 [H2 Hneq%not_elem_of_singleton]%elem_of_difference.
+    intros ->. apply Hneq.
+    f_equal. by eapply bij_set_injective.
+  Qed.
+
+End bij_set.
