theories/Commons/Values.v
@@ -1,0 +1,17 @@
+From RSL Require Import Prelude.
+
+Definition loc : Type := positive.
+
+Variant val : Type :=
+| VInt (v: Z)
+| VBool (b : bool)
+| VPtr (l : loc)
+| VUndef.
+
+Definition val_eq (loc_eq : loc -> loc -> Prop) (v1 v2 : val) :=
+  match v1, v2 with
+  | VInt i1, VInt i2 => i1 = i2
+  | VBool b1, VBool b2 => b1 = b2
+  | VPtr p1, VPtr p2 => loc_eq p1 p2
+  | _, _ => False
+  end.
