theories/Logic.v
@@ -1,2 +1,0 @@
-From RSL Require Export Logic.Logic.
-From RSL Require Export Logic.Memory.
