theories/Logic/BI.v
@@ -1,0 +1,179 @@
+From RSL Require Import Prelude.
+
+From iris.bi Require Export bi.
+From iris.proofmode Require Export proofmode.
+
+From RSL.Logic Require Import rPropDef.
+
+Section BI_def.
+  Import rProp_primitive.
+
+  Local Instance rPropDef_dist : Dist rPropDef := fun _ => equiv.
+
+  (** ** BI Mixin *)
+
+  Lemma rProp_bi_mixin :
+    BiMixin
+      rPropDef_entails
+      rPropDef_empty
+      rPropDef_pure
+      rPropDef_and
+      rPropDef_or
+      rPropDef_impl
+      rPropDef_forall
+      rPropDef_exist
+      rPropDef_sep
+      rPropDef_wand.
+  Proof using Type.
+    constructor.
+    - by apply entails_po.
+    - by apply equiv_entails.
+    - unfold dist, rPropDef_dist; intros _.
+      by apply pure_ne.
+    - unfold dist, rPropDef_dist; intros _.
+      by apply and_ne.
+    - unfold dist, rPropDef_dist; intros _.
+      by apply or_ne.
+    - unfold dist, rPropDef_dist; intros _.
+      by apply impl_ne.
+    - unfold dist, rPropDef_dist; intros ? _.
+      by apply forall_ne.
+    - unfold dist, rPropDef_dist; intros ? _.
+      by apply exist_ne.
+    - unfold dist, rPropDef_dist; intros _.
+      by apply sep_ne.
+    - unfold dist, rPropDef_dist; intros _.
+      by apply wand_ne.
+    - by apply pure_intro.
+    - by apply pure_elim.
+    - by apply and_elim_l.
+    - by apply and_elim_r.
+    - by apply and_intro.
+    - by apply or_intro_l.
+    - by apply or_intro_r.
+    - by apply or_elim.
+    - by apply impl_intro.
+    - by apply impl_elim.
+    - by apply forall_intro.
+    - by apply forall_elim.
+    - by apply exist_intro.
+    - by apply exist_elim.
+    - by apply sep_mono.
+    - by apply emp_sep_1.
+    - by apply emp_sep_2.
+    - by apply sep_comm.
+    - by apply sep_assoc.
+    - by apply wand_intro.
+    - by apply wand_elim.
+  Qed.
+
+  Definition bi_persistently_mixin :
+    BiPersistentlyMixin
+      rPropDef_entails
+      rPropDef_empty
+      rPropDef_and
+      rPropDef_exist
+      rPropDef_sep
+      rPropDef_persistently.
+  Proof using Type.
+    pose proof rProp_bi_mixin as H. revert H.
+    apply bi_persistently_mixin_discrete.
+    - done.
+    - unseal. intros Q Φ H. destruct (H ∅ ∅) as [x Hx]. { done. }
+      exists x. intros ? ?.
+      by intros [-> ->].
+    - intros P. by unseal.
+  Qed.
+
+  (** ** Later connective *)
+
+  Definition bi_later_mixin :
+    BiLaterMixin
+      rPropDef_entails
+      rPropDef_pure
+      rPropDef_or
+      rPropDef_impl
+      rPropDef_forall
+      rPropDef_exist
+      rPropDef_sep
+      rPropDef_persistently
+      rPropDef_later.
+  Proof using Type.
+    pose proof rProp_bi_mixin as H. revert H.
+    apply bi_later_mixin_id. by unseal.
+  Qed.
+
+  (** ** RProp is a BI *)
+
+  Global Canonical Structure rProp : bi :=
+    {|
+      bi_car := rPropDef;
+      bi_dist := dist;
+      bi_equiv := equiv;
+      bi_entails := rPropDef_entails;
+      bi_emp := rPropDef_empty;
+      bi_pure := rPropDef_pure;
+      bi_and := rPropDef_and;
+      bi_or := rPropDef_or;
+      bi_impl := rPropDef_impl;
+      bi_forall := rPropDef_forall;
+      bi_exist := rPropDef_exist;
+      bi_sep := rPropDef_sep;
+      bi_wand := rPropDef_wand;
+      bi_persistently := rPropDef_persistently;
+      bi_later := rPropDef_later;
+      bi_ofe_mixin := discrete_ofe_mixin equiv_equiv;
+      bi_cofe_aux := discrete_cofe equiv_equiv;
+      bi_bi_mixin := rProp_bi_mixin;
+      bi_bi_persistently_mixin := bi_persistently_mixin;
+      bi_bi_later_mixin := bi_later_mixin;
+    |}.
+
+  (** Extra BI instances *)
+
+  Global Instance rProp_persistently_forall : BiPersistentlyForall rProp.
+  Proof.
+    intros A Ψ.
+    unfold bi_entails, bi_persistently, bi_forall. simpl. unseal.
+    intros mt ms H ? ? [-> ->] a. by apply H.
+  Qed.
+
+  Global Instance rProp_pure_forall : BiPureForall rProp.
+  Proof.
+    intros A φ.
+    unfold bi_entails, bi_pure, bi_forall. simpl. unseal.
+    intros mt ms H a. apply H.
+  Qed.
+
+End BI_def.
+
+Notation "'⌜' φ '⌟'" :=
+  (bi_affinely (bi_pure φ%type%stdpp))%I
+    (at level 0, φ constr at level 200) : bi_scope.
+
+Ltac unseal :=
+  repeat (
+      unfold
+        bi_entails,
+        bi_pure,
+        bi_and,
+        bi_or,
+        bi_impl,
+        bi_forall,
+        bi_exist,
+        bi_sep,
+        bi_wand,
+        bi_persistently,
+        bi_later,
+        bi_emp_valid,
+        bi_intuitionistically,
+        bi_absorbingly,
+        bi_affinely,
+        bi_wand_iff,
+        bi_emp,
+        bi_iff;
+      rProp_primitive.unseal;
+      simpl
+    ).
+
+Ltac unseal_in H := revert H; unseal; intro H.
