theories/Logic/MemInj.v
@@ -1,0 +1,188 @@
+From RSL Require Import Prelude.
+
+From RSL.Commons Require Export BijSet.
+From RSL.Logic Require Export PointsTo.
+
+Definition related (j: gset (loc * loc)) (lt ls: loc) :=
+  (ls, lt) ∈ j.
+
+Definition same_val (j: gset (loc * loc)) := val_eq (related j).
+
+Lemma same_val_mono j j' vt vs :
+  j ⊆ j' ->
+  same_val j vt vs ->
+  same_val j' vt vs.
+Proof using Type.
+  destruct vt as [], vs as []; simpl; auto.
+  unfold related. by auto.
+Qed.
+
+Definition in_inj (j : gset (loc * loc)) (E: gmap loc loc) :=
+  ∀ ls lt, E !! ls = Some lt -> (ls, lt) ∈ j.
+
+Lemma in_inj_mono j j' E : j ⊆ j' -> in_inj j E -> in_inj j' E.
+Proof using Type.
+  by intros Hincl Hinj lt ls H; auto.
+Qed.
+
+Lemma in_inj_extend j E lt ls :
+  related j lt ls ->
+  in_inj j E ->
+  in_inj j (<[ls:=lt]> E).
+Proof using Type.
+  intros Hrel Hinj ls' lt'.
+  rewrite lookup_insert.
+  case_decide as He.
+  - intros H. by inv H.
+  - intros HeE. by apply Hinj.
+Qed.
+
+Lemma in_inj_remove j E ls :
+  in_inj j E ->
+  in_inj j (delete ls E).
+Proof using Type.
+  intros Hinj ls' lt'.
+  rewrite lookup_delete.
+  case_decide as He.
+  - intros H. by inv H.
+  - intros HeE. by apply Hinj.
+Qed.
+
+Definition mem_inj (j : gset (loc * loc)) (E: gmap loc loc) : rProp :=
+  (
+    ⌜bij_set j⌟ ∗
+    ⌜in_inj j E⌟ ∗
+    [∗ set] '(ls, lt) ∈ j,
+      ∃ vt vs,
+        ⌜same_val j vt vs⌟ ∗
+        if (E !! ls)
+        then emp
+        else lt →ₜ vt ∗ ls →ₛ vs
+  )%I.
+
+Lemma inj_empty : ⊢ mem_inj ∅ ∅.
+Proof using Type.
+  unfold mem_inj.
+  iSplit.
+  { iPureIntro. by apply bij_set_empty. }
+  iSplit.
+  { easy. }
+  { by iApply big_sepS_empty. }
+Qed.
+
+Lemma inj_insert_exploit j E lt ls vt vs :
+  E !! ls = None ->
+  (∀ ls' lt', E !! ls' = Some lt' -> lt' ≠ lt) ->
+  mem_inj j E -∗
+  lt →ₜ vt -∗
+  ls →ₛ vs -∗
+  ⌜same_val j vt vs⌟ -∗
+  mem_inj ({[ (ls, lt) ]} ∪ j) E.
+Proof using Type.
+  iIntros (Hls Hlt) "(%Hbij & %HE & Hin) Ht Hs %H".
+
+  iAssert (⌜∀ lt', (ls, lt') ∉ j⌝)%I with "[Hin Hs]" as "%Hs".
+  {
+    iIntros (lt' Hej).
+    iDestruct (big_sepS_delete _ _ _ Hej with "Hin") as "[Hcond H]".
+    rewrite Hls.
+    iDestruct "Hcond" as (vt' vs') "(_ & Ht' & Hs')".
+    by iDestruct (src_points_to_unique with "Hs Hs'") as "%Hneq".
+  }
+
+  iAssert (⌜∀ ls', (ls', lt) ∉ j⌝)%I with "[Hin Ht]" as "%Ht".
+  {
+    iIntros (ls' Hej).
+    iDestruct (big_sepS_delete _ _ _ Hej with "Hin") as "[Hcond H]".
+    destruct (E !! ls') as [lt'| ] eqn:HeE.
+    - assert (lt = lt'). { by eapply bij_set_functional; eauto. }
+      subst lt'. exfalso. by eapply Hlt.
+    - iDestruct "Hcond" as (vt' vs') "(_ & Ht' & Hs')".
+      by iDestruct (tgt_points_to_unique with "Ht Ht'") as "%Hneq".
+  }
+
+  iSplitR.
+  { iPureIntro. by apply bij_set_extend. }
+  iSplitR.
+  { iPureIntro. apply in_inj_mono with j; auto. by apply union_subseteq_r. }
+  iApply big_sepS_union.
+  { intros [] He%elem_of_singleton Hj. inv He. by apply (Ht ls). }
+  iSplitR "Hin".
+  - iApply big_sepS_singleton. rewrite Hls.
+    iExists vt, vs. iFrame. iPureIntro.
+    apply same_val_mono with j; auto.
+    by apply union_subseteq_r.
+  - iApply (big_sepS_impl with "Hin").
+    iModIntro. iIntros ([lt'' ls''] Hin) "(%vt' & %vs' & %Hsame & Hcond)".
+    iExists vt', vs'. iFrame.
+    iPureIntro.
+    apply same_val_mono with j; auto.
+    by apply union_subseteq_r.
+Qed.
+
+Lemma inj_insert j lt ls vt vs :
+  mem_inj j ∅ -∗
+  lt →ₜ vt -∗
+  ls →ₛ vs -∗
+  ⌜same_val j vt vs⌟ -∗
+  mem_inj ({[ (ls, lt) ]} ∪ j) ∅.
+Proof using Type. by apply inj_insert_exploit. Qed.
+
+Lemma inj_exploit j E lt ls :
+  related j lt ls ->
+  E !! ls = None ->
+  mem_inj j E -∗
+  ∃ vt vs,
+    lt →ₜ vt ∗
+    ls →ₛ vs ∗
+    ⌜same_val j vt vs⌟ ∗
+    mem_inj j (<[ls := lt]>E).
+Proof using Type.
+  iIntros (Hrel HnE) "(%Hbij & %HE & Hin)".
+  iDestruct (big_sepS_delete _ _ _ Hrel with "Hin") as "[Hpair Hin]".
+  iDestruct "Hpair" as (vt vs) "[%Hsame Hcond]".
+  rewrite HnE.
+  iDestruct "Hcond" as "[Ht Hs]".
+  iExists vt, vs. iFrame.
+  iSplitR. { done. }
+
+  iSplitR. { done. }
+  iSplitR. { iPureIntro. by apply in_inj_extend. }
+
+  iApply (big_sepS_delete _ _ _ Hrel).
+  iSplitR.
+  - iExists vt, vs. by rewrite lookup_insert decide_True.
+  - iApply (big_sepS_impl with "Hin").
+    iModIntro.
+    iIntros ([ls' lt'] Hneq).
+    iIntros "(%vt' & %vs' & Hsame & Hcond)".
+    iExists vt', vs'. iFrame.
+    assert (ls ≠ ls') by (by eapply bij_set_diff_fst_neq).
+    now rewrite lookup_insert_ne.
+Qed.
+
+Lemma inj_release j E lt ls vt vs:
+  E !! ls = Some lt ->
+  same_val j vt vs ->
+  mem_inj j E -∗
+  lt →ₜ vt -∗
+  ls →ₛ vs -∗
+  mem_inj j (delete ls E).
+Proof using Type.
+  iIntros (HE Hsame) "(%Hbij & %Hinj & Hin) Ht Hs".
+  iSplitR. { done. }
+  iSplitR. { iPureIntro. by apply in_inj_remove. }
+  assert (Hin: (ls, lt) ∈ j) by (now apply Hinj).
+  iDestruct (big_sepS_delete _ _ _ Hin with "Hin") as "[H Hin]".
+  rewrite HE.
+  iDestruct "H" as (vt' vs' Hsame') "_".
+  iApply (big_sepS_delete _ _ _ Hin).
+  iSplitL "Ht Hs".
+  - iExists vt, vs. rewrite lookup_delete_eq. by iFrame.
+  - iApply (big_sepS_impl with "Hin"). clear vt' vs' Hsame'.
+    iModIntro.
+    iIntros ([ls' lt'] Hin') "(%vt' & %vs' & Hsame & H)".
+    iExists vt', vs'. iFrame.
+    assert (ls ≠ ls') by (by eapply bij_set_diff_fst_neq).
+    now rewrite lookup_delete_ne.
+Qed.
