theories/Logic/PointsTo.v
@@ -1,0 +1,46 @@
+From RSL Require Import Prelude.
+
+From RSL.Commons Require Export Memory.
+
+From RSL.Logic Require Export BI.
+From RSL.Logic Require Import rPropDef.
+
+Definition tgt_points_to loc v : rProp :=
+  {| rProp_holds mt ms := mt = {[ loc := v ]} ∧ ms = ∅ |}.
+
+Definition src_points_to loc v : rProp :=
+  {| rProp_holds mt ms := mt = ∅ ∧ ms = {[ loc := v ]} |}.
+
+Notation "l '→ₜ' v" :=
+  (tgt_points_to l%positive v%Z)
+    (at level 70, no associativity, format "l →ₜ v") : bi_scope.
+
+Notation "l '→ₛ' v" :=
+  (src_points_to l%positive v%Z)
+    (at level 70, no associativity, format "l →ₛ v") : bi_scope.
+
+Lemma tgt_points_to_unique lt1 lt2 v1 v2:
+  lt1 →ₜ v1 -∗
+  lt2 →ₜ v2 -∗
+  ⌜lt1 ≠ lt2⌝.
+Proof.
+  unfold tgt_points_to, src_points_to.
+  unseal.
+  intros ? ? [-> ->] ? ? _ _ [H1 ->] ? ? Hd _ [H2 _] ->.
+  simpl in *.
+  apply map_disjoint_union_r in Hd as [_ Hd].
+  apply map_disjoint_dom in Hd. subst. set_solver.
+Qed.
+
+Lemma src_points_to_unique ls1 ls2 v1 v2:
+  ls1 →ₛ v1 -∗
+  ls2 →ₛ v2 -∗
+  ⌜ls1 ≠ ls2⌝.
+Proof.
+  unfold tgt_points_to, src_points_to.
+  unseal.
+  intros ? ? [-> ->] ? ? _ _ [-> H1] ? ? _ Hd [_ H2] ->.
+  simpl in *.
+  apply map_disjoint_union_r in Hd as [_ Hd].
+  apply map_disjoint_dom in Hd. subst. set_solver.
+Qed.
