theories/RTL/TargetRules.v
@@ -1,145 +1,165 @@
-(* From RSL Require Import RelLogic Prelude. *)
+From RSL Require Import Prelude.
 
-(* From Coinduction Require Import all. *)
+From RSL.Logic Require Export Logic.
+From RSL.Simulations Require Export FreeSimRules.
+From RSL.RTL Require Export RTL Semantics Notations.
 
-(* From RSL Require Import Simulations.FreeSim. *)
-(* From RSL Require Import Simulations.FreeSimRules. *)
+Import RTLNotations.
 
-(* From RSL Require Import RTL.RTL. *)
-(* From RSL Require Import RTL.Semantics. *)
-(* From RSL Require Import RTL.Notations. *)
-(* From RSL Require Import RTL.SimRules. *)
+Section TargetRulesDef.
+  Let Λₜ : lang := rtl_lang.
+  Let Λₛ : lang := rtl_lang.
+  Context (Pₜ: prog Λₜ) (Pₛ: prog Λₛ).
 
-(* From RSL Require Import Tactics.Memory. *)
+  Abbreviation sim_lfp := (sim_lfp Pₜ Pₛ).
 
-(* Import RTLNotations. *)
+  Notation
+    "'[' C ']' st '<{' j ',' i '}=' ss '{{' Q '}}'" :=
+    (sim_lfp C st j i ss Q%I)
+      (at level 0,
+       st at level 99,
+       ss at level 99,
+       Q at level 200,
+       no associativity).
 
-(* Section TargetRulesDef. *)
-(*   Let Λₜ : lang := rtl_lang. *)
-(*   Let Λₛ : lang := rtl_lang. *)
-(*   Context (Pₜ: prog Λₜ) (Pₛ: prog Λₛ). *)
+  Ltac smap :=
+    rewrite ?map_union_empty ?map_empty_union ?map_union_assoc;
+    try done.
 
-(*   Abbreviation fsim := (fsim WfNat WfNat Pₜ Pₛ). *)
+  Lemma target_nop C ct ft pct ρt j i ss Q :
+    ∀ pc,
+    ft@pct is <<{ nop -> pc }>> ->
+    [C] (ct, State ft pc ρt) <{1+j, i}= ss {{ Q }} -∗
+    [C] (ct, State ft pct ρt) <{j, i}= ss {{ Q }}.
+  Proof using Type.
+    intros pc Hpc.
+    unseal. intros ? ? [-> ->] ? ? _ _ Hsim. smap.
 
-(*   Notation *)
-(*     "'[' C ']' ρ '⊢' ft '@' pct  '<{' j ',' i '}=' fs '@' pcs '{{' Q '}}'" := *)
-(*     (sim Pₜ Pₛ C ρ ft pct j i fs pcs Q%rlogic) *)
-(*       (at level 0, ft at level 0, fs at level 0, no associativity). *)
+    apply FTargetSteps.
+    - eexists. by econstructor.
+    - intros t Hstep. inv Hstep.
+      eexists. now apply Hsim.
+  Qed.
 
-(*   Notation *)
-(*     "'[' C ']' ρ '⊢' '{{' P '}}' ft '@' pct  '<{' j ',' i '}=' fs '@' pcs '{{' Q '}}'" := *)
-(*     (hoare Pₜ Pₛ C ρ P%rlogic ft pct j i fs pcs Q%rlogic) *)
-(*       (at level 0, ft at level 0, fs at level 0, no associativity). *)
+  Lemma target_ret C ct ft pct ρt j i ss Q :
+    ∀ r v,
+    ft@pct is <<{ ret r }>> ->
+    ρt@r ⇒ v ->
+    [C] (ct, ReturnState v) <{1+j, i}= ss {{ Q }} -∗
+    [C] (ct, State ft pct ρt) <{j, i}= ss {{ Q }}.
+  Proof using Type.
+    intros r v Hpc Hr.
+    unseal. intros ? ? [-> ->] ? ? _ _ Hsim.
+    smap.
 
-(*   Lemma target_nop C ρₜ ρₛ P fₜ pcₜ j i fₛ pcₛ Q : *)
-(*     ∀ pc, *)
-(*     fₜ@pcₜ is <<{ nop -> pc }>> -> *)
-(*     [C] (ρₜ, ρₛ) ⊢ {{ P }} fₜ @ pc <{1+j, i}= fₛ @ pcₛ {{ Q }} -> *)
-(*     [C] (ρₜ, ρₛ) ⊢ {{ P }} fₜ @ pcₜ <{j, i}= fₛ @ pcₛ {{ Q }}. *)
-(*   Proof using Type. *)
-(*     intros pc Hpc H. *)
-(*     intros ? ? Hemp Ψ mtPre msPre ? ? Hpre mtPost msPost ? ? Hpost. *)
+    eapply FTargetSteps.
+    - eexists. by econstructor.
+    - intros t' Hstep. inv Hstep. simregs.
+      eexists. by apply Hsim.
+  Qed.
 
-(*     eapply FTargetSteps. *)
-(*     - eexists. econstructor; eassumption. *)
-(*     - intros t Hstep. inv Hstep. *)
-(*       eexists. now apply H. *)
-(*   Qed. *)
+  Lemma target_op C ct ft pct ρt j i ss Q :
+    ∀ pc dst op regs args v,
+    ft@pct is <<{ dst := @op regs -> pc }>> ->
+    ρt @ regs ⇒ args ->
+    eval_op op args = Some v ->
+    [C] (ct, State ft pc (⟦dst ⇐ v⟧ρt)) <{1+j, i}= ss {{ Q }} -∗
+    [C] (ct, State ft pct ρt) <{j, i}= ss {{ Q }}.
+  Proof using Type.
+    intros pc dst op regs args v Hpc Hargs Hv.
+    unseal. intros ? ? [-> ->] ? ? _ _ Hsim. smap.
 
-(*   Lemma target_op C ρₜ ρₛ P fₜ pcₜ j i fₛ pcₛ Q : *)
-(*     ∀ pc dst op regs args v, *)
-(*     fₜ@pcₜ is <<{ dst := @op regs -> pc }>> -> *)
-(*     ρₜ @ regs ⇒ args -> *)
-(*     eval_op op args = Some v -> *)
-(*     [C] (⟦dst ⇐ v⟧ρₜ, ρₛ) ⊢ {{ P }} fₜ @ pc <{1+j, i}= fₛ @ pcₛ {{ Q }} -> *)
-(*     [C] (ρₜ, ρₛ) ⊢ {{ P }} fₜ @ pcₜ <{j, i}= fₛ @ pcₛ {{ Q }}. *)
-(*   Proof using Type. *)
-(*     intros pc dst op regs args v Hpc Hargs Hv H. *)
-(*     intros ? ? Hemp Ψ mtPre msPre ? ? Hpre mtPost msPost ? ? Hpost. *)
+    eapply FTargetSteps.
+    - eexists. by econstructor.
+    - intros t Hstep. inv Hstep. simregs.
+      eexists. now apply Hsim.
+  Qed.
 
-(*     eapply FTargetSteps. *)
-(*     - eexists. econstructor; eassumption || reflexivity. *)
-(*     - intros t Hstep. inv Hstep. simregs. *)
-(*       eexists. now apply H. *)
-(*   Qed. *)
+  Lemma target_load C ct ft pct ρt j i ss Q :
+    ∀ pc dst src l v,
+    ft@pct is <<{ dst := !src -> pc }>> ->
+    ρt @ src ⇒ VPtr l ->
+    (l →ₜ v -∗
+     [C] (ct, State ft pc (⟦dst ⇐ v⟧ρt)) <{1+j, i}= ss {{ Q }}) -∗
+    l →ₜ v -∗
+    [C] (ct, State ft pct ρt) <{j, i}= ss {{ Q }}.
+  Proof using Type.
+    intros pc dst src l v Hpc Haddr.
+    unseal.
+    intros ? ? [-> ->] mtP msP _ _ Hsim. smap.
+    intros ? ? ? _ [-> ->]. smap.
 
-(*   Lemma target_load C ρₜ ρₛ P fₜ pcₜ j i fₛ pcₛ Q : *)
-(*     ∀ pc dst src addr v, *)
-(*     fₜ@pcₜ is <<{ dst := !src -> pc }>> -> *)
-(*     ρₜ @ src ⇒ addr -> *)
-(*     [C] (⟦dst ⇐ v⟧ρₜ, ρₛ) ⊢ {{ addr →ₜ v ∗ P }} fₜ @ pc <{1+j, i}= fₛ @ pcₛ {{ Q }} -> *)
-(*     [C] (ρₜ, ρₛ) ⊢ {{ addr →ₜ v ∗ P }} fₜ @ pcₜ <{j, i}= fₛ @ pcₛ {{ Q }}. *)
-(*   Proof using Type. *)
-(*     intros pc dst src addr v Hpc Haddr H. *)
-(*     intros ? ? Hemp Ψ mtPre msPre ? ? Hpre mtPost msPost ? ? Hpost. *)
+    decompose_map_disjoint.
 
-(*     destruct Hpre as (mtAddr & msAddr & mtP & msP & ? & ? & ? & ? & Hm & HP). *)
-(*     destruct Hm as ((l & Hl & Ht) & Hs). *)
+    eapply FTargetSteps.
+    - eexists. eapply exec_Iload; try eassumption.
+      + rewrite get_at_union_right; last done.
+        by apply get_at_singl.
+      + reflexivity.
+    - intros t Hstep.
+      inv Hstep as [ | | | ? ? ? ? ? ? ? ? ? ? ? ? ? Hget | | | | | ].
+      simregs.
+      rewrite get_at_union_right in Hget; last done.
+      rewrite get_at_singl in Hget. inv Hget.
 
-(*     eapply FTargetSteps. *)
-(*     - eexists. eapply exec_Iload; try eassumption. *)
-(*       + subst. now simget. *)
-(*       + reflexivity. *)
-(*     - subst. *)
-(*       intros t Hstep. *)
-(*       inv Hstep. simregs. simget. subst. *)
+      eexists.
+      replace msP with (msP ∪ ∅) by smap.
+      apply Hsim; smap; by solve_map_disjoint.
+  Qed.
 
-(*       eexists. apply H; try solve_map_disjoint. *)
-(*       eexists _, ∅, mtP, msP. repeat split; eauto. *)
-(*       exists l. now split. *)
-(*   Qed. *)
+  Lemma target_store C ct ft pct ρt j i ss Q :
+    ∀ pc dst src l v old,
+    ft@pct is <<{ !dst := src -> pc }>> ->
+    ρt @ dst ⇒ VPtr l ->
+    ρt @ src ⇒ v ->
+    (l →ₜ v -∗
+     [C] (ct, State ft pc ρt) <{1+j, i}= ss {{ Q }}) -∗
+    l →ₜ old -∗
+    [C] (ct, State ft pct ρt) <{j, i}= ss {{ Q }}.
+  Proof using Type.
+    intros pc dst src l v old Hpc Haddr Hv.
+    unseal.
+    intros ? ? [-> ->] mtP msP _ _ Hsim. smap.
+    intros ? ? ? _ [-> ->]. smap.
 
-(*   Lemma target_store C ρₜ ρₛ P fₜ pcₜ j i fₛ pcₛ Q : *)
-(*     ∀ pc dst src addr v old, *)
-(*     fₜ@pcₜ is <<{ !dst := src -> pc }>> -> *)
-(*     ρₜ @ dst ⇒ addr -> *)
-(*     ρₜ @ src ⇒ v -> *)
-(*     [C] (ρₜ, ρₛ) ⊢ {{ addr →ₜ v ∗ P }} fₜ @ pc <{1+j, i}= fₛ @ pcₛ {{ Q }} -> *)
-(*     [C] (ρₜ, ρₛ) ⊢ {{ addr →ₜ old ∗ P }} fₜ @ pcₜ <{j, i}= fₛ @ pcₛ {{ Q }}. *)
-(*   Proof using Type. *)
-(*     intros pc dst src addr v old Hpc Haddr Hv H. *)
-(*     intros ? ? Hemp Ψ mtPre msPre ? ? Hpre mtPost msPost ? ? Hpost. *)
+    decompose_map_disjoint.
 
-(*     destruct Hpre as (mtAddr & msAddr & mtP & msP & ? & ? & ? & ? & Hm & HP). *)
-(*     destruct Hm as ((l & Hl & Ht) & Hs). *)
+    eapply FTargetSteps.
+    - eexists. eapply exec_Istore; try eassumption.
+      eapply set_at_some.
+      rewrite get_at_union_right; last done.
+      by apply get_at_singl.
+    - intros t Hstep.
+      inv Hstep as [ | | | | ? ? ? ? ? ? ? ? ? ? ? ? ? ? Hset | | | | ].
+      simregs.
+      erewrite set_at_some in Hset.
+      + rewrite insert_union_r in Hset; last done.
+        rewrite insert_singleton_eq in Hset.
+        inv Hset.
 
-(*     eapply FTargetSteps. *)
-(*     - eexists. eapply exec_Istore; try eassumption. *)
-(*       subst. *)
-(*       erewrite (set_at_some  _ _ _ _ _ Hl) by simget. *)
-(*       rewrite !alter_union_right, !alter_union_left, alter_singleton by solve_map_disjoint. *)
-(*       reflexivity. *)
-(*     - intros t Hstep. *)
-(*       inv Hstep. *)
-(*       simregs. *)
-(*       erewrite (set_at_some  _ _ _ _ _ Hl) in * by simget. *)
-(*       rewrite !alter_union_right, !alter_union_left, alter_singleton *)
-(*                 in * by solve_map_disjoint. *)
-(*       rewrite inj_some in *. *)
+        eexists.
+        replace msP with (msP ∪ ∅) by smap.
+        apply Hsim; smap; by solve_map_disjoint.
+      + rewrite get_at_union_right; last done.
+        by apply get_at_singl.
+  Qed.
 
-(*       subst. decompose_map_disjoint. *)
-(*       eexists. apply H; try solve_map_disjoint. *)
-(*       eexists _, ∅, mtP, msP. repeat split; eauto. *)
-(*       + solve_map_disjoint. *)
-(*       + solve_map_disjoint. *)
-(*       + exists l. now split. *)
-(*   Qed. *)
+  Lemma target_if C ct ft pct ρt j i ss Q :
+    ∀ pc_true pc_false reg b,
+    ft@pct is <<{ if reg then goto pc_true else goto pc_false }>> ->
+    ρt @ reg ⇒ VBool b ->
+    let pc := if b then pc_true else pc_false in
+    [C] (ct, State ft pc ρt) <{1+j, i}= ss {{ Q }} -∗
+    [C] (ct, State ft pct ρt) <{j, i}= ss {{ Q }}.
+  Proof using Type.
+    intros pc_true pc_false reg b pc Hpc.
+    unseal.
+    intros ? ? [-> ->] ? ? _ _ Hsim. smap.
 
-(*   Lemma target_if C ρₜ ρₛ P fₜ pcₜ j i fₛ pcₛ Q : *)
-(*     ∀ pc_true pc_false reg v pc, *)
-(*     fₜ@pcₜ is <<{ if reg then goto pc_true else goto pc_false }>> -> *)
-(*     ρₜ @ reg ⇒ v -> *)
-(*     (if (v =? 0)%Z then pc_true else pc_false) = pc -> *)
-(*     [C] (ρₜ, ρₛ) ⊢ {{ P }} fₜ @ pc <{1+j, i}= fₛ @ pcₛ {{ Q }} -> *)
-(*     [C] (ρₜ, ρₛ) ⊢ {{ P }} fₜ @ pcₜ <{j, i}= fₛ @ pcₛ {{ Q }}. *)
-(*   Proof using Type. *)
-(*     intros pc_true pc_false reg v pc Hpc Hv Hnext_pc H. *)
-(*     intros ? ? Hemp Ψ mtPre msPre ? ? Hpre mtPost msPost ? ? Hpost. *)
+    apply FTargetSteps.
+    - eexists. by econstructor.
+    - intros t Hstep. inv Hstep. simregs.
+      eexists. now apply Hsim.
+  Qed.
 
-(*     eapply FTargetSteps. *)
-(*     - eexists. econstructor; eassumption || reflexivity. *)
-(*     - intros t Hstep. inv Hstep. simregs. *)
-(*       eexists. now apply H. *)
-(*   Qed. *)
-
-(* End TargetRulesDef. *)
+End TargetRulesDef.
